\input{preamble}

\FBOX{
11.6
Solve Equation 11.17 to second order in perturbation theory,
for the general case $c_a(0)=a$, $c_b(0)=b$.
}

Zeroth order:
\begin{equation*}
c_a(t)=a,\quad c_b(t)=b
\end{equation*}

First order:
\begin{equation*}
\begin{aligned}
\dot c_a^{(1)}(t)&=\left[-\frac{i}{\hbar}H_{ab}'e^{-i\omega_0t}c_b\right]_{c_b=b}
&&=-\frac{ib}{\hbar}H_{ab}'e^{-i\omega_0t}
\\
\dot c_b^{(1)}(t)&=\left[-\frac{i}{\hbar}H_{ba}'e^{i\omega_0t}c_a\right]_{c_a=a}
&&=-\frac{ia}{\hbar}H_{ba}'e^{i\omega_0t}
\end{aligned}
\tag{1}
\end{equation*}

Hence
\begin{equation*}
\begin{aligned}
c_a^{(1)}&=a+\int_0^t\dot c_a^{(1)}(t')\,dt'
& &=a-\frac{ib}{\hbar}\int_0^tH_{ab}'(t')e^{-i\omega_0t'}\,dt'
\\
c_b^{(1)}&=b+\int_0^t\dot c_b^{(1)}(t')\,dt'
& &=b-\frac{ia}{\hbar}\int_0^tH_{ba}'(t')e^{i\omega_0t'}\,dt'
\end{aligned}
\tag{2}
\end{equation*}

Second order:
\begin{equation*}
\begin{aligned}
\dot c_a^{(2)}(t)&=\left[-\frac{i}{\hbar}H_{ab}'e^{-i\omega_0t}c_b\right]_{c_b=c_b^{(1)}}
&&=-\frac{ib}{\hbar}H_{ab}'e^{-i\omega_0t}-\frac{a}{\hbar^2}H_{ab}'e^{-i\omega_0t}
\int_0^tH_{ba}'(t')e^{i\omega_0t'}\,dt'
\\
\dot c_b^{(2)}(t)&=\left[-\frac{i}{\hbar}H_{ba}'e^{i\omega_0t}c_a\right]_{c_a=c_a^{(1)}}
&&=-\frac{ia}{\hbar}H_{ba}'e^{i\omega_0t}-\frac{b}{\hbar^2}H_{ba}'e^{i\omega_0t}
\int_0^tH_{ab}'(t')e^{-i\omega_0t'}\,dt'
\end{aligned}
\tag{3}
\end{equation*}

Hence
\begin{multline*}
c_a^{(2)}=a+\int_0^t\dot c_a^{(2)}(t')\,dt'
\\
=a-\frac{ib}{\hbar}\int_0^tH_{ab}'(t')e^{-i\omega_0t'}\,dt'
-\frac{a}{\hbar^2}\int_0^tH_{ab}'(t')e^{-i\omega_0t'}
\left[\int_0^{t'}H_{ba}'(t'')e^{i\omega_0t''}\,dt''\right]\,dt'
\tag{4}
\end{multline*}

and
\begin{multline*}
c_b^{(2)}=b+\int_0^t\dot c_b^{(2)}(t')\,dt'
\\
=b-\frac{ia}{\hbar}\int_0^tH_{ba}'(t')e^{i\omega_0t'}\,dt'
-\frac{b}{\hbar^2}\int_0^tH_{ba}'(t')e^{i\omega_0t'}
\left[\int_0^{t'}H_{ab}'(t'')e^{-i\omega_0t''}\,dt''\right]\,dt'
\tag{5}
\end{multline*}

\end{document}
