\input{preamble}

\FBOX{
11.14
From the commutators of $L_z$ with $x$, $y$, and $z$ (Equation 4.122):
\begin{equation*}
[L_z,x]=i\hbar y,\quad[L_z,y]=-i\hbar x,\quad[L_z,z]=0,\tag{11.77}
\end{equation*}

obtain the selection rule for $\Delta m$ and Equation 11.76.
{\it Hint:} Sandwich each commutator between
$\langle n'l'm'|$ and $|nlm\rangle$.
}

Recall that
\begin{equation*}
L_z|nlm\rangle=m\hbar|nlm\rangle,\quad
\langle n'l'm'|L_z=m'\hbar\langle n'l'm'|
\end{equation*}

Hence
\begin{align*}
\langle n'l'm'|(L_zx-xL_z)|nlm\rangle
&=(m'-m)\hbar\langle n'l'm'|x|nlm\rangle=i\hbar\langle n'l'm'|y|nlm\rangle
\\
\langle n'l'm'|(L_zy-yL_z)|nlm\rangle
&=(m'-m)\hbar\langle n'l'm'|y|nlm\rangle=-i\hbar\langle n'l'm'|x|nlm\rangle
\\
\langle n'l'm'|(L_zz-zL_z)|nlm\rangle
&=(m'-m)\hbar\langle n'l'm'|z|nlm\rangle=0
\end{align*}

For clarity, let
\begin{equation*}
\Delta m=m'-m,\quad X=\langle n'l'm'|x|nlm\rangle,\quad
Y=\langle n'l'm'|y|nlm\rangle,\quad Z=\langle n'l'm'|z|nlm\rangle
\end{equation*}

Then
\begin{align*}
\Delta m&=\frac{iY}{X}=-\frac{iX}{Y},\quad\Delta mZ=0
\end{align*}


\end{document}
