\input{preamble}

\FBOX{
11.7
Calculate $c_a(t)$ and $c_b(t)$, to second order, for the perturbation
in Problem 11.3. Compare your answer with the exact result.
}

\begin{equation*}
\dot c_a=-\frac{i}{\hbar}H_{ab}'e^{-i\omega_0t}c_b,\quad
\dot c_b=-\frac{i}{\hbar}H_{ba}'e^{i\omega_0t}c_a
\tag{11.17}
\end{equation*}

First order:
\begin{align*}
\dot c_a^{(1)}&=-\frac{i}{\hbar}H_{ab}'e^{-i\omega_0t}c_b\bigg|_{c_b=0}
&&=0
\\
\dot c_b^{(1)}&=-\frac{i}{\hbar}H_{ba}'e^{i\omega_0t}c_a\bigg|_{c_a=1}
&&=-\frac{i}{\hbar}H_{ba}'e^{i\omega_0t}
\end{align*}

Hence
\begin{align*}
c_a^{(1)}(t)&=c_a(0)+\int_0^t\dot c_a^{(1)}(t')\,dt'
&&=1
\\
c_b^{(1)}(t)&=c_b(0)+\int_0^t\dot c_b^{(1)}(t')\,dt'
&&=\frac{H_{ba}'}{\hbar\omega_0}\left(1-e^{i\omega_0t}\right)
\end{align*}

Second order:
\begin{align*}
\dot c_a^{(2)}&=-\frac{i}{\hbar}H_{ab}'e^{-i\omega_0t}c_b\bigg|_{c_b=c_b^{(1)}}
& &=\frac{iH_{ab}'H_{ba}'}{\hbar^2\omega_0}\left(1-e^{-i\omega_0t}\right)
\\
\dot c_b^{(2)}&=-\frac{i}{\hbar}H_{ba}'e^{i\omega_0t}c_a\bigg|_{c_a=c_a^{(1)}}
& &=-\frac{i}{\hbar}H_{ba}'e^{i\omega_0t}
\end{align*}

Hence
\begin{align*}
c_a^{(2)}(t)&=c_a(0)+\int_0^t\dot c_a^{(2)}(t')\,dt'
&&=1+\frac{H_{ab}'H_{ba}'}{\hbar^2\omega_0^2}
\left(i\omega_0t+e^{-i\omega_0t}-1\right)
\\
c_b^{(2)}(t)&=c_b(0)+\int_0^t\dot c_b^{(2)}(t')\,dt'
&&=\frac{H_{ba}'}{\hbar\omega_0}\left(1-e^{i\omega_0t}\right)
\end{align*}

\end{document}
