\input{preamble}

\fbox{\parbox{\dimexpr\linewidth-2\fboxsep-2\fboxrule}{
Exercise 9.1.
Derive Eq.~9.7 by plugging Eq.~9.6 into Eq.~9.5.
}}

\bigskip
We are given
\begin{gather*}
-\frac{\hbar^2}{2m}\frac{\partial^2\psi(x)}{\partial x^2}=E\psi(x)\tag{9.5}
\\[1ex]
\psi(x)=\exp\left(\frac{ipx}{\hbar}\right)\tag{9.6}
\\[1ex]
E=\frac{p^2}{2m}\tag{9.7}
\end{gather*}

For the $\psi(x)$ given in equation (9.6) we have
\begin{equation*}
\frac{\partial^2}{\partial x^2}\psi(x)
=-\frac{p^2}{\hbar^2}\psi(x)
\tag{1}
\end{equation*}

Substitute (1) into (9.5) to obtain
\begin{equation*}
\frac{p^2}{2m}\psi(x)=E\psi(x)
\end{equation*}

Hence
\begin{equation*}
\frac{p^2}{2m}=E
\end{equation*}

\end{document}
