\input{preamble}

\fbox{\parbox{\dimexpr\linewidth-2\fboxsep-2\fboxrule}{
24-4.
Suppose $A_1$, $A_2$, $A_3$ and $K_1$, $K_2$, $K_3$ are matrices
that represent projections of two vector quantities
and $B$ is a matrix that represents a scalar
quantity, so $B$ commutes with $J_1$, $J_2$, $J_3$ and each
set of matrices $A_1$, $A_2$, $A_3$ and $K_1$, $K_2$, $K_3$ satisfies
the commutation relations with $J_1$, $J_2$, $J_3$
that characterize rotations of a vector quantity.
Show that each set of matrices
\begin{equation*}
A_1+K_1,\quad A_2+K_2,\quad A_3+K_3
\end{equation*}

and
\begin{equation*}
BA_1,\quad BA_2,\quad BA_3
\end{equation*}

satisfies the commutation relations with $J_1$, $J_2$,
$J_3$ that characterize rotations of a vector quantity.
Show that the matrix
\begin{equation*}
A_1K_1+A_2K_2+A_3K_3
\end{equation*}

commutes with $J_1$, $J_2$, $J_3$.
}}

\bigskip
For $J_1$ we have
\begin{align*}
(A_1+K_1)J_1-J_1(A_1+K_1)&=0
\\
(A_2+K_2)J_1-J_1(A_2+K_2)&=-i(A_3+K_3)
\\
(A_3+K_3)J_1-J_1(A_3+K_3)&=i(A_2+K_2)
\end{align*}

and
\begin{align*}
BA_1J_1-J_1BA_1&=0
\\
BA_2J_1-J_1BA_2&=-iBA_3
\\
BA_3J_1-J_1BA_3&=iBA_2
\end{align*}

For $J_2$ we have
\begin{align*}
(A_1+K_1)J_2-J_2(A_1+K_1)&=i(A_3+K_3)
\\
(A_2+K_2)J_2-J_2(A_2+K_2)&=0
\\
(A_3+K_3)J_2-J_2(A_3+K_3)&=-i(A_1+K_1)
\end{align*}

and
\begin{align*}
BA_1J_2-J_2BA_1&=iBA_3
\\
BA_2J_2-J_2BA_2&=0
\\
BA_3J_2-J_2BA_3&=-iBA_1
\end{align*}

For $J_3$ we have
\begin{align*}
(A_1+K_1)J_3-J_3(A_1+K_1)&=-i(A_2+K_2)
\\
(A_2+K_2)J_3-J_3(A_2+K_2)&=i(A_1+K_1)
\\
(A_3+K_3)J_3-J_3(A_3+K_3)&=0
\end{align*}

and
\begin{align*}
BA_1J_3-J_3BA_1&=-iBA_2
\\
BA_2J_3-J_3BA_2&=iBA_1
\\
BA_3J_3-J_3BA_3&=0
\end{align*}

Note that
\begin{align*}
[AK,J]&=AKJ-JAK
\\
&=AKJ-AJK+AJK-JAK
\\
&=A[K,J]+[A,J]K
\end{align*}

Hence for $J_1$ we have
\begin{align*}
[A_1K_1,J_1]&=0
\\
[A_2K_2,J_1]&=-iA_2K_3-iA_3K_2
\\
[A_3K_3,J_1]&=iA_3K_2+iA_2K_3
\end{align*}

Hence
\begin{equation*}
(A_1K_1+A_2K_2+A_3K_3)J_1-J_1(A_1K_1+A_2K_2+A_3K_3)=0
\end{equation*}

Similarly for $J_2$ and $J_3$.

\end{document}
