\input{preamble}

\fbox{\parbox{\dimexpr\linewidth-2\fboxsep-2\fboxrule}{
18-4.
Show that
\begin{equation*}
R^2H-HR^2=-2\hbar\omega R^2
\end{equation*}

and
\begin{equation*}
HS^2-S^2H=-2\hbar\omega S^2
\end{equation*}

Use these and the result of Problem 17-5 to find
$\langle R^2\rangle$, $\langle S^2\rangle$, $\langle Q^2\rangle$,
$\langle P^2\rangle$ and
$(\frac{1}{2})m\omega^2\langle Q^2\rangle$,
$(1/2m)\langle P^2\rangle$ for the state where
the oscillator energy has the value $(n+\frac{1}{2})\hbar\omega$.
}}

\bigskip
From problem 18-3
\begin{equation*}
RH-HR=-\hbar\omega R
\end{equation*}

Hence
\begin{align*}
R^2H-RHR=-\hbar\omega R^2
\\
RHR-HR^2=-\hbar\omega R^2
\end{align*}

Add together to obtain
\begin{equation*}
R^2H-HR^2=-2\hbar\omega R^2
\end{equation*}

From problem 18-3
\begin{equation*}
HS-SH=-\hbar\omega S
\end{equation*}

Hence
\begin{align*}
HS^2-SHS=-\hbar\omega S^2
\\
SHS-S^2H=-\hbar\omega S^2
\end{align*}

Add together to obtain
\begin{equation*}
HS^2-S^2H=-2\hbar\omega S^2
\end{equation*}

If $H$ has a definite value then by the result of problem 17-5 we have
\begin{equation*}
\langle R^2\rangle=0,\quad\langle S^2\rangle=0
\end{equation*}

Noting that
\begin{equation*}
Q^2=\tfrac{1}{4}(R+S)^2
\end{equation*}

we have
\begin{equation*}
\langle Q^2\rangle=\tfrac{1}{4}\left(\langle R^2\rangle
+\langle RS\rangle+\langle SR\rangle+\langle S^2\rangle\right)
\end{equation*}

If $H$ has a definite value then
\begin{equation*}
\langle Q^2\rangle=\tfrac{1}{4}\left(\langle RS\rangle+\langle SR\rangle\right)\tag{1}
\end{equation*}

For the oscillator energy we have
\begin{equation*}
\langle H\rangle=\tfrac{1}{4}m\omega^2(\langle RS\rangle+\langle SR\rangle)
=\left(n+\tfrac{1}{2}\right)\hbar\omega
\tag{2}
\end{equation*}

Substitute (2) into (1) to obtain
\begin{equation*}
\langle Q^2\rangle=\left(n+\tfrac{1}{2}\right)\frac{\hbar}{m\omega}
\end{equation*}

Hence
\begin{equation*}
\tfrac{1}{2}m\omega^2\langle Q^2\rangle=\left(n+\tfrac{1}{2}\right)\frac{\hbar\omega}{2}
\end{equation*}

Noting that
\begin{equation*}
P^2=-\tfrac{1}{4}m^2\omega^2(R-S)^2
\end{equation*}

we have
\begin{equation*}
\langle P^2\rangle=-\tfrac{1}{4}m^2\omega^2\left(\langle R^2\rangle
-\langle RS\rangle-\langle SR\rangle
+\langle S^2\rangle\right)
\end{equation*}

If $H$ has a definite value then
\begin{equation*}
\langle P^2\rangle=\tfrac{1}{4}m^2\omega^2(\langle RS\rangle+\langle SR\rangle)\tag{3}
\end{equation*}

Substitute (2) into (3) to obtain
\begin{equation*}
\langle P^2\rangle=\left(n+\tfrac{1}{2}\right)m\hbar\omega
\end{equation*}

Hence
\begin{equation*}
\frac{1}{2m}\langle P^2\rangle=\left(n+\tfrac{1}{2}\right)\frac{\hbar\omega}{2}
\end{equation*}

\end{document}
