\input{preamble}

\fbox{\parbox{\dimexpr\linewidth-2\fboxsep-2\fboxrule}{
17-6.
Suppose $K$ and $L$ represent real quantities.
Show
\begin{equation*}
\langle K^2\rangle\langle L^2\rangle
\ge\left|\tfrac{1}{2}\langle KL+LK\rangle\right|^2
\end{equation*}

for any state. This implies $\langle KL+LK\rangle$ is 0
if either $\langle K^2\rangle$ or $\langle L^2\rangle$ is 0.
}}

\bigskip
From p.~131
\begin{equation*}
\langle K^2\rangle\langle L^2\rangle
\ge|\langle KL\rangle|^2
\tag{1}
\end{equation*}

Write $\langle KL\rangle$ as
\begin{equation*}
\langle KL\rangle=i(-i)\tfrac{1}{2}\langle KL+LK\rangle+\tfrac{1}{2}\langle KL-LK\rangle
\end{equation*}

Note that for real numbers $x$ and $y$
\begin{equation*}
|x+iy|^2=x^2+y^2\ge y^2,\quad y^2=|iy|^2
\end{equation*}

Hence for
\begin{equation*}
y=(-i)\tfrac{1}{2}\langle KL+LK\rangle
\end{equation*}

we have
\begin{equation*}
|\langle KL\rangle|^2\ge|iy|^2,\quad|iy|^2=\left|\tfrac{1}{2}\langle KL+LK\rangle\right|^2
\end{equation*}

Combine with (1) to obtain
\begin{equation*}
\langle K^2\rangle\langle L^2\rangle\ge|\langle KL\rangle|^2
\ge\left|\tfrac{1}{2}\langle KL+LK\rangle\right|^2
\end{equation*}

Hence
\begin{equation*}
\langle K^2\rangle\langle L^2\rangle\ge\left|\tfrac{1}{2}\langle KL+LK\rangle\right|^2
\end{equation*}

\end{document}
