\input{preamble}

\fbox{\parbox{\dimexpr\linewidth-2\fboxsep-2\fboxrule}{
20-3.
Use the result of the last problem to calculate
\begin{equation*}
L_3(Q_1^2+Q_2^2+Q_3^2)-(Q_1^2+Q_2^2+Q_3^2)L_3
\end{equation*}

and
\begin{equation*}
L_3(P_1^2+P_2^2+P_3^2)-(P_1^2+P_2^2+P_3^2)L_3
\end{equation*}

Both of these can be done the same way $J_3J^2-J^2J_3$ was.
}}

\bigskip
Start with
\begin{align*}
[L_3,Q^2]&=L_3(Q_1^2+Q_2^2+Q_3^2)-(Q_1^2+Q_2^2+Q_3^2)L_3
\\
&=L_3Q_1Q_1-Q_1Q_1L_3+L_3Q_2Q_2-Q_2Q_2L_3+L_3Q_3Q_3-Q_3Q_3L_3
\end{align*}

By problem 20-2
\begin{align*}
Q_1L_3&=L_3Q_1-i\hbar Q_2
\\
Q_2L_3&=L_3Q_2+i\hbar Q_1
\\
Q_3L_3&=L_3Q_3
\end{align*}

Substitute from problem 20-2.
\begin{align*}
[L_3,Q^2]
&=L_3Q_1Q_1-Q_1(L_3Q_1-i\hbar Q_2)+L_2Q_2Q_2-Q_2(L_3Q_2+i\hbar Q_1)
\\
&=(L_3Q_1-Q_1L_3)Q_1+(L_3Q_2-Q_2L_3)Q_2
\\
&=i\hbar Q_2Q_1-i\hbar Q_1Q_2
\\
&=0
\end{align*}

Repeat with $P$ substituted for $Q$.

\end{document}
