\input{preamble}

\fbox{\parbox{\dimexpr\linewidth-2\fboxsep-2\fboxrule}{
17-1.
Find
\begin{gather*}
\left\langle(\Sigma_1-\langle\Sigma_1\rangle)^2\right\rangle,
\\
\left\langle(\Sigma_2-\langle\Sigma_2\rangle)^2\right\rangle,
\end{gather*}

and
\begin{equation*}
\left\langle(\Sigma_3-\langle\Sigma_3\rangle)^2\right\rangle
\end{equation*}

for a state where the quantity represented by $\Sigma_3$ has
the definite value 1.
}}

\bigskip
If $\Sigma_3$ has the definite value 1 then $\langle\Sigma_3\rangle=1$ and by
\begin{equation*}
\langle\Sigma_1\rangle^2+\langle\Sigma_2\rangle^2+\langle\Sigma_3\rangle^2\le1
\end{equation*}

we have
\begin{equation*}
\langle\Sigma_2\rangle=0,\quad\langle\Sigma_3\rangle=0
\end{equation*}

Hence
\begin{align*}
\left\langle(\Sigma_1-\langle\Sigma_1\rangle)^2\right\rangle
&=\left\langle\Sigma_1^2\right\rangle=1
\\
\left\langle(\Sigma_2-\langle\Sigma_2\rangle)^2\right\rangle
&=\left\langle\Sigma_2^2\right\rangle=1
\end{align*}

and
\begin{align*}
\left\langle(\Sigma_3-\langle\Sigma_3\rangle)^2\right\rangle
&=\left\langle(\Sigma_3-1)^2\right\rangle
\\
&=\left\langle\Sigma_3^2-2\Sigma_3+1\right\rangle
\\
&=2-2\langle\Sigma_3\rangle
\\
&=0
\end{align*}

\end{document}
