\input{preamble}

\fbox{\parbox{\dimexpr\linewidth-2\fboxsep-2\fboxrule}{
17-2.
For every case where $A$ and $B$ are two of the matrices
$\Sigma_1$, $\Sigma_2$, $\Sigma_3$ verify that the uncertainty relation
\begin{equation*}
\left\langle(A-\langle A\rangle)^2\right\rangle
\left\langle(B-\langle B\rangle)^2\right\rangle
\ge\left|\tfrac{1}{2}\langle AB-BA\rangle\right|^2
\end{equation*}

holds for the state where the quantity represented
by $\Sigma_3$ has the definite value 1.
}}

\bigskip
From problem 17-1, when $\Sigma_3$ has the definite value 1 we have
\begin{equation*}
\langle\Sigma_1\rangle=0,\quad
\langle\Sigma_2\rangle=0,\quad
\langle\Sigma_3\rangle=1
\end{equation*}

and
\begin{align*}
\left\langle(\Sigma_1-\langle\Sigma_1\rangle)^2\right\rangle&=1
\\
\left\langle(\Sigma_2-\langle\Sigma_2\rangle)^2\right\rangle&=1
\\
\left\langle(\Sigma_3-\langle\Sigma_3\rangle)^2\right\rangle&=0
\end{align*}

For the case $A=B$ we have
\begin{equation*}
\left\langle(A-\langle A\rangle)^2\right\rangle
\left\langle(B-\langle B\rangle)^2\right\rangle
=\text{0 or 1}
\end{equation*}

and
\begin{equation*}
\left|\tfrac{1}{2}\langle AB-BA\rangle\right|^2=0
\end{equation*}

hence the formula holds for this case.

\bigskip
For the case $A=\Sigma_1$ and $B=\Sigma_2$ we have
\begin{equation*}
\left\langle(A-\langle A\rangle)^2\right\rangle
\left\langle(B-\langle B\rangle)^2\right\rangle=1
\end{equation*}

and
\begin{align*}
\left|\tfrac{1}{2}\langle AB-BA\rangle\right|^2
&=\left|\tfrac{1}{2}\langle\Sigma_1\Sigma_2-\Sigma_2\Sigma_1\rangle\right|^2
\\
&=\left|\tfrac{1}{2}\langle i\Sigma_3+i\Sigma_3\rangle\right|^2
\\
&=1
\end{align*}

hence the formula holds for this case.

\bigskip
For the case $A=\Sigma_1$ and $B=\Sigma_3$ we have
\begin{equation*}
\left\langle(A-\langle A\rangle)^2\right\rangle
\left\langle(B-\langle B\rangle)^2\right\rangle=0
\end{equation*}

and
\begin{align*}
\left|\tfrac{1}{2}\langle AB-BA\rangle\right|^2
&=\left|\tfrac{1}{2}\langle\Sigma_1\Sigma_3-\Sigma_3\Sigma_1\rangle\right|^2
\\
&=\left|\tfrac{1}{2}\langle -i\Sigma_2-i\Sigma_2\rangle\right|^2
\\
&=0
\end{align*}

hence the formula holds for this case.

\bigskip
The remaining cases are trivial variations.

\end{document}
