\input{preamble}

\fbox{\parbox{\dimexpr\linewidth-2\fboxsep-2\fboxrule}{
12.4.1
Show that for
$|s\rangle=\cos(\theta/2)|{\uparrow}\rangle
+\exp(i\phi)\sin(\theta/2)|{\downarrow}\rangle$
\begin{equation*}
\langle s|\hat{\boldsymbol\sigma}|s\rangle
=\mathbf i\sin\theta\cos\phi+\mathbf j\sin\theta\sin\phi+\mathbf k\cos\theta
\end{equation*}
}}

\bigskip
Noting that
\begin{align*}
\langle s|\hat\sigma_x|s\rangle&=\sin\theta\cos\phi
\\
\langle s|\hat\sigma_y|s\rangle&=\sin\theta\sin\phi
\\
\langle s|\hat\sigma_z|s\rangle&=\cos\theta
\end{align*}

we have
\begin{equation*}
\langle s|\hat{\boldsymbol\sigma}|s\rangle=
\mathbf i\langle s|\hat\sigma_x|s\rangle+\mathbf j\langle s|\hat\sigma_y|s\rangle
+\mathbf k\langle s|\hat\sigma_z|s\rangle
=\mathbf i\sin\theta\cos\phi+\mathbf j\sin\theta\sin\phi+\mathbf k\cos\theta
\end{equation*}

\end{document}
