\input{preamble}

\fbox{\parbox{\dimexpr\linewidth-2\fboxsep-2\fboxrule}{
15.6.2
Using the results of Prob.~15.6.1, find an expression for the
expectation value of the ``position'' $\xi_\lambda$ for the
coherent state in Eq.~(15.94) in terms of $\bar n$, $\omega_\lambda$
and time $t$.
}}

\bigskip
The expectation of $\hat\xi_\lambda$ for the coherent state is
\begin{equation*}
\langle\hat\xi_\lambda\rangle=\langle\Psi_{\lambda\bar n}|\hat\xi_\lambda|\Psi_{\lambda\bar n}\rangle
\end{equation*}

The operator $\hat\xi_\lambda$ is given by equation (15.78).
\begin{equation*}
\hat\xi_\lambda\equiv\frac{1}{\sqrt2}\left(\hat a_\lambda+\hat a_\lambda^\dag\right)
\tag{15.78}
\end{equation*}

Hence
\begin{equation*}
\langle\hat\xi_\lambda\rangle
=\frac{1}{\sqrt2}
\langle\Psi_{\lambda\bar n}|
\left(\hat a_\lambda+\hat a_\lambda^\dag\right)
|\Psi_{\lambda\bar n}\rangle
\end{equation*}

Expand the right-hand side.
\begin{equation*}
\langle\hat\xi_\lambda\rangle
=\frac{1}{\sqrt2}
\langle\Psi_{\lambda\bar n}|
\hat a_\lambda
|\Psi_{\lambda\bar n}\rangle
+\frac{1}{\sqrt2}
\langle\Psi_{\lambda\bar n}|
\hat a_\lambda^\dag
|\Psi_{\lambda\bar n}\rangle
\tag{1}
\end{equation*}

From problem 15.6.1 we have
\begin{equation*}
\hat a_\lambda|\Psi_{\lambda\bar n}\rangle
=\sqrt{\bar n}\exp(-i\omega_\lambda t)|\Psi_{\lambda\bar n}\rangle
\tag{2}
\end{equation*}

It follows that
\begin{equation*}
\langle\Psi_{\lambda\bar n}|\hat a_\lambda^\dag
=\left(\hat a_\lambda|\Psi_{\lambda\bar n}\rangle\right)^\dag
=\sqrt{\bar n}\exp(i\omega_\lambda t)\langle\Psi_{\lambda\bar n}|
\tag{3}
\end{equation*}

Substitute (2) and (3) into (1) to obtain
\begin{equation*}
\langle\hat\xi_\lambda\rangle
=\sqrt{\frac{\bar n}{2}}\exp(-i\omega_\lambda t)
\langle\Psi_{\lambda\bar n}|\Psi_{\lambda\bar n}\rangle
+\sqrt{\frac{\bar n}{2}}\exp(i\omega_\lambda t)
\langle\Psi_{\lambda\bar n}|\Psi_{\lambda\bar n}\rangle
\end{equation*}

Noting that $\langle\Psi_{\lambda\bar n}|\Psi_{\lambda\bar n}\rangle=1$ we have
\begin{equation*}
\langle\hat\xi_\lambda\rangle
=\sqrt{\frac{\bar n}{2}}\exp(-i\omega_\lambda t)+\sqrt{\frac{\bar n}{2}}\exp(i\omega_\lambda t)
\end{equation*}

Finally, by the identity
\begin{equation*}
2\cos(\omega_\lambda t)=\exp(-i\omega_\lambda t)+\exp(i\omega_\lambda t)
\end{equation*}

we have
\begin{equation*}
\langle\hat\xi_\lambda\rangle=\sqrt{2\bar n}\cos(\omega_\lambda t)
\end{equation*}

\end{document}
