\input{preamble}

\fbox{\parbox{\dimexpr\linewidth-2\fboxsep-2\fboxrule}{
15.5.1
Find the commutator $[\hat\xi_\lambda,\hat\pi_\lambda]$
starting from the operator definitions
\begin{equation*}
\hat\xi_\lambda\equiv\frac{1}{\sqrt2}
\left(\hat a_\lambda+\hat a_\lambda^\dag\right)
\quad\text{and}\quad
\hat\pi_\lambda\equiv\frac{i}{\sqrt2}
\left(\hat a_\lambda^\dag-\hat a_\lambda\right)
\end{equation*}
}}

\bigskip
We have
\begin{equation*}
\hat\xi_\lambda\hat\pi_\lambda=\frac{i}{2}
\left(\hat a_\lambda\hat a_\lambda^\dag-\hat a_\lambda \hat a_\lambda
+\hat a_\lambda^\dag\hat a_\lambda^\dag-\hat a_\lambda^\dag\hat a_\lambda\right)
\tag{1}
\end{equation*}
and
\begin{equation*}
\hat\pi_\lambda\hat\xi_\lambda=\frac{i}{2}
\left(\hat a_\lambda^\dag\hat a_\lambda+\hat a_\lambda^\dag\hat a_\lambda^\dag
-\hat a_\lambda\hat a_\lambda-\hat a_\lambda\hat a_\lambda^\dag\right)
\tag{2}
\end{equation*}

Subtract (2) from (1) to obtain the commutator.
\begin{equation*}
[\hat\xi_\lambda,\hat\pi_\lambda]
=i\left(\hat a_\lambda\hat a_\lambda^\dag
-\hat a_\lambda^\dag\hat a_\lambda\right)
\end{equation*}

From
\begin{equation*}
[\hat a_\lambda,\hat a_\lambda^\dag]
=\hat a_\lambda\hat a_\lambda^\dag-\hat a_\lambda^\dag\hat a_\lambda=1
\end{equation*}
we have
\begin{equation*}
[\hat\xi_\lambda,\hat\pi_\lambda]=i
\end{equation*}

\end{document}
