\input{preamble}

\fbox{\parbox{\dimexpr\linewidth-2\fboxsep-2\fboxrule}{
15.1.1
Prove the relation
\begin{equation*}
[\hat a,\hat a^\dag]=\hat a\hat a^\dag-\hat a^\dag\hat a=1
\end{equation*}
for the harmonic oscillator raising and lowering operators, starting from their definitions
\begin{equation*}
\hat a^\dag=\frac{1}{\sqrt2}\left(-\frac{d}{d\xi}+\xi\right)
\quad\text{and}\quad
\hat a=\frac{1}{\sqrt2}\left(\frac{d}{d\xi}+\xi\right)
\end{equation*}
}}

\bigskip
For $\hat a\hat a^\dag$ we have
\begin{equation*}
\hat a\hat a^\dag\psi=\frac{1}{2}\left(\frac{d}{d\xi}+\xi\right)\left(-\frac{d}{d\xi}+\xi\right)\psi
\end{equation*}

Expand the right-hand side.
\begin{align*}
\hat a\hat a^\dag\psi
%&=\frac{1}{2}\left(\frac{d}{d\xi}+\xi\right)\left(-\frac{d}{d\xi}\psi+\xi\psi\right)
%\\
&=\frac{1}{2}\left(-\frac{d^2}{d\xi^2}\psi+\frac{d}{d\xi}(\xi\psi)-\xi\frac{d}{d\xi}\psi+\xi^2\psi\right)
\\
&=\frac{1}{2}\left(-\frac{d^2}{d\xi^2}\psi+\psi+\xi^2\psi\right)
\tag{1}
\end{align*}

For $\hat a^\dag\hat a$ we have
\begin{equation*}
\hat a^\dag\hat a\psi=\frac{1}{2}\left(-\frac{d}{d\xi}+\xi\right)\left(\frac{d}{d\xi}+\xi\right)\psi
\end{equation*}

Expand the right-hand side.
\begin{align*}
\hat a^\dag\hat a\psi
%&=\frac{1}{2}\left(-\frac{d}{d\xi}+\xi\right)\left(\frac{d}{d\xi}\psi+\xi\psi\right)
%\\
&=\frac{1}{2}\left(-\frac{d^2}{d\xi^2}\psi-\frac{d}{d\xi}(\xi\psi)+\xi\frac{d}{d\xi}\psi+\xi^2\psi\right)
\\
&=\frac{1}{2}\left(-\frac{d^2}{d\xi^2}\psi-\psi+\xi^2\psi\right)
\tag{2}
\end{align*}

Subtract (2) from (1).
\begin{equation*}
\hat a\hat a^\dag\psi-\hat a^\dag\hat a\psi=\frac{1}{2}\psi-\left(-\frac{1}{2}\psi\right)=\psi
\end{equation*}

Hence
\begin{equation*}
[\hat a,\hat a^\dag]=1
\end{equation*}

\end{document}
