\input{preamble}

\fbox{\parbox{\dimexpr\linewidth-2\fboxsep-2\fboxrule}{
15.6.1
Show that the coherent state in Eq.~(15.94) is an eigenstate of the
annihilation operator $\hat a_\lambda$, with eigenvalue
$\sqrt{\bar n}\exp(-i\omega_\lambda t)$.
}}

\bigskip
This is equation (15.94).
\begin{equation*}
|\Psi_{\lambda\bar n}\rangle=\sum_{n_\lambda=0}^\infty
c_{\lambda\bar nn}
\exp\left[-i\left(n_\lambda+\tfrac{1}{2}\right)\omega_\lambda t\right]
|n_\lambda\rangle
\tag{15.94}
\end{equation*}

We will also need equation (15.95).
\begin{equation*}
c_{\lambda\bar nn}
=\sqrt{\frac{\bar n^{n_\lambda}\exp(-\bar n)}{n_\lambda!}}
\tag{15.95}
\end{equation*}

We want to show that
\begin{equation*}
\hat a_\lambda|\Psi_{\lambda\bar n}\rangle
=\sqrt{\bar n}\exp(-i\omega_\lambda t)|\Psi_{\lambda\bar n}\rangle
\end{equation*}

Apply operator $\hat a_\lambda$ to state $|\Psi_{\lambda\bar n}\rangle$ to obtain
\begin{equation*}
\hat a_\lambda|\Psi_{\lambda\bar n}\rangle
=\sum_{n_\lambda=0}^\infty
c_{\lambda\bar nn}
\exp\left[-i\left(n_\lambda+\tfrac{1}{2}\right)\omega_\lambda t\right]
\sqrt{n_\lambda}|n_\lambda-1\rangle
\end{equation*}

The $n_\lambda=0$ term vanishes hence the sum can start from $n_\lambda=1$.
\begin{equation*}
\hat a_\lambda|\Psi_{\lambda\bar n}\rangle
=\sum_{n_\lambda=1}^\infty
c_{\lambda\bar nn}
\exp\left[-i\left(n_\lambda+\tfrac{1}{2}\right)\omega_\lambda t\right]
\sqrt{n_\lambda}|n_\lambda-1\rangle
\end{equation*}

The $\sqrt{n_\lambda}$ cancels with the denominator in $c_{\lambda\bar nn}$.
\begin{equation*}
\hat a_\lambda|\Psi_{\lambda\bar n}\rangle
=\sum_{n_\lambda=1}^\infty
\sqrt{\frac{\bar n^{n_\lambda}\exp(-\bar n)}{(n_\lambda-1)!}}
\exp\left[-i\left(n_\lambda+\tfrac{1}{2}\right)\omega_\lambda t\right]
|n_\lambda-1\rangle
\end{equation*}

On the right-hand side, factor out $\sqrt{\bar n}\exp(-i\omega_\lambda t)$.
\begin{multline*}
\hat a_\lambda|\Psi_{\lambda\bar n}\rangle=
\\
\sqrt{\bar n}\exp(-i\omega_\lambda t)
\sum_{n_\lambda=1}^\infty
\sqrt{\frac{\bar n^{n_\lambda-1}\exp(-\bar n)}{(n_\lambda-1)!}}
\exp\left[-i\left(n_\lambda-\tfrac{1}{2}\right)\omega_\lambda t\right]
|n_\lambda-1\rangle
\end{multline*}

Substitute $n_\lambda+1$ for index $n_\lambda$.
\begin{equation*}
\hat a_\lambda|\Psi_{\lambda\bar n}\rangle
=\sqrt{\bar n}\exp(-i\omega_\lambda t)
\sum_{n_\lambda=0}^\infty
\sqrt{\frac{\bar n^{n_\lambda}\exp(-\bar n)}{n_\lambda!}}
\exp\left[-i\left(n_\lambda+\tfrac{1}{2}\right)\omega_\lambda t\right]
|n_\lambda\rangle
\end{equation*}

Hence
\begin{equation*}
\hat a_\lambda|\Psi_{\lambda\bar n}\rangle=\sqrt{\bar n}\exp(-i\omega_\lambda t)|\Psi_{\lambda\bar n}\rangle
\end{equation*}

\end{document}
