\input{preamble}

\fbox{\parbox{\dimexpr\linewidth-2\fboxsep-2\fboxrule}{
11.1.1
Consider a single barrier of thickness $L$, with height $V$ much larger than
the energy $E$ of an
electron wave incident on the left of the barrier.
Presume the barrier is thick enough that the amount
of wave reflected back from the right hand side of the barrier to the left is
essentially negligible.
Show that the fraction $\eta$ of incident electrons transmitted by this
barrier can be written approximately as
\begin{equation*}
\eta\approx\frac{16k^2\kappa^2}{\left(k^2+\kappa^2\right)^2}
\exp(-2\kappa L)
\end{equation*}

where $k=(2m_oE/\hbar^2)^{1/2}$ and $\kappa=[2m_o(V-E)/\hbar^2]^{1/2}$.
[Note: use the expression of the form $\eta=|F|^2/|A|^2$ where $F$ and $A$
are the amplitudes of the transmitted and incident waves respectively;
otherwise the algebra becomes much more involved.]
}}

\bigskip
From figure 11.1
\begin{align*}
\psi_L(z)&=Ae^{ikz}+Be^{-ikz}
\\
\psi_B(z)&=Ce^{-\kappa z}+De^{\kappa z}
\\
\psi_R(z)&=Fe^{ikz}
\end{align*}

From the boundary condition $\psi_B(L)=\psi_R(L)$
\begin{equation*}
Ce^{-\kappa L}+De^{\kappa L}=Fe^{ikL}
\tag{1}
\end{equation*}

From the boundary condition $\psi'_B(L)=\psi'_R(L)$
\begin{equation*}
-\kappa Ce^{-\kappa L}+\kappa De^{\kappa L}=ikFe^{ikL}
\tag{2}
\end{equation*}

Add $-\kappa$ times (1) to (2) to obtain
\begin{equation*}
-2\kappa Ce^{-\kappa L}=(-\kappa+ik)Fe^{ikL}
\end{equation*}

Hence
\begin{equation*}
C=\frac{\kappa-ik}{2\kappa}F\exp(ikL+\kappa L)
\end{equation*}

Add $\kappa$ times (1) to (2) to obtain
\begin{equation*}
2\kappa De^{\kappa L}=(\kappa+ik)Fe^{ikL}
\end{equation*}

Hence
\begin{equation*}
D=\frac{\kappa+ik}{2\kappa}F\exp(ikL-\kappa L)
\end{equation*}

Note that
\begin{equation*}
\frac{|C|}{|D|}=\exp(2\kappa L)
\end{equation*}

Hence $|C|\gg|D|$ for $2\kappa L\gg1$.

\bigskip
From the boundary condition $\psi_L(0)=\psi_B(0)$
\begin{equation*}
A+B=C+D
\tag{3}
\end{equation*}

From the boundary condition $\psi'_L(0)=\psi'_B(0)$
\begin{equation*}
ikA-ikB=-\kappa C+\kappa D
\tag{4}
\end{equation*}

Add $ik$ times (3) to (4) to obtain
\begin{equation*}
2ikA=(ik-\kappa)C+(ik+\kappa)D
\end{equation*}

Hence
\begin{equation*}
A=\frac{ik-\kappa}{2ik}C+\frac{ik+\kappa}{2ik}D
\end{equation*}

Substitute for $C$ and use the approximation $D=0$.
\begin{equation*}
A=\frac{(ik-\kappa)(\kappa-ik)}{4ik\kappa}F\exp(ikL+\kappa L)
\end{equation*}

Hence
\begin{equation*}
\frac{F}{A}=\frac{4ik\kappa}{(ik-\kappa)(\kappa-ik)}\exp(-ikL-\kappa L)
\end{equation*}

and
\begin{equation*}
\eta=\left|\frac{F}{A}\right|^2=\frac{16k^2\kappa^2}{\left(k^2+\kappa^2\right)^2}\exp(-2\kappa L)
\end{equation*}

\end{document}
