\input{preamble}

\fbox{\parbox{\dimexpr\linewidth-2\fboxsep-2\fboxrule}{
15.7.1
Consider a set of modes of the electromagnetic field in which the electric
field is polarized along the $x$ direction and the magnetic field is polarized
in the $y$ direction.
Restricting consideration only to those modes, find the simplest expression
you can for the commutation relation $[\hat E_x,\hat B_y]$
for this multimode field.
}}

\bigskip
Consider the following formulas.
\begin{align*}
\hat{\mathbf E}(\mathbf r,t)
&=i\sum_\lambda\left(\hat a_\lambda-\hat a_\lambda^\dag\right)
\sqrt\frac{\hbar\omega_\lambda}{2\epsilon_0}
\mathbf u_\lambda(\mathbf r)
\tag{15.132}
\\
\hat{\mathbf B}(\mathbf r,t)
&=\sum_\lambda\left(\hat a_\lambda+\hat a_\lambda^\dag\right)
\sqrt\frac{\hbar\omega_\lambda\mu_0}{2}
\mathbf v_\lambda(\mathbf r)
\tag{15.135}
\end{align*}

By hypothesis we have for the polarization vectors
\begin{equation*}
\mathbf u_\lambda(\mathbf r)=\begin{pmatrix}1\\0\\0\end{pmatrix},
\quad
\mathbf v_\lambda(\mathbf r)=\begin{pmatrix}0\\1\\0\end{pmatrix}
\end{equation*}

Hence
\begin{align*}
\hat E_x(\mathbf r,t)
&=i\sum_\lambda\left(\hat a_\lambda-\hat a_\lambda^\dag\right)
\sqrt\frac{\hbar\omega_\lambda}{2\epsilon_0}
\\
\hat B_y(\mathbf r,t)
&=\sum_\lambda\left(\hat a_\lambda+\hat a_\lambda^\dag\right)
\sqrt\frac{\hbar\omega_\lambda\mu_0}{2}
\end{align*}

It follows that
\begin{align*}
\hat E_x\hat B_y&=i\frac{\hbar}{2}\sqrt{\frac{\mu_0}{\epsilon_0}}\sum_\lambda\omega_\lambda
\left(\hat a_\lambda-\hat a_\lambda^\dag\right)
\left(\hat a_\lambda+\hat a_\lambda^\dag\right)
\tag{1}
\\
\hat B_y\hat E_x&=i\frac{\hbar}{2}\sqrt{\frac{\mu_0}{\epsilon_0}}\sum_\lambda\omega_\lambda
\left(\hat a_\lambda+\hat a_\lambda^\dag\right)
\left(\hat a_\lambda-\hat a_\lambda^\dag\right)
\tag{2}
\end{align*}

Subtract (2) from (1) to obtain the commutator.
\begin{equation*}
[\hat E_x,\hat B_y]
=i\frac{\hbar}{2}\sqrt{\frac{\mu_0}{\epsilon_0}}\sum_\lambda\omega_\lambda
\left(2\hat a_\lambda\hat a_\lambda^\dag-2\hat a_\lambda^\dag\hat a_\lambda\right)
\end{equation*}

Recalling that $\hat a_\lambda\hat a_\lambda^\dag-\hat a_\lambda^\dag\hat a_\lambda=1$ we have
\begin{equation*}
[\hat E_x,\hat B_y]
=i\hbar\sqrt\frac{\mu_0}{\epsilon_0}\sum_\lambda\omega_\lambda
\end{equation*}

\end{document}
