\input{preamble}

\FBOX{
4-2. Calculate $\langle x\rangle$, $\langle x^2\rangle$,
and $\sigma_x$, as well as $\langle p\rangle$, $\langle p^2\rangle$,
and $\sigma_p$, for the normalized wavefunction
\begin{equation*}
\psi(x)=\sqrt{\frac{2a^3}{\pi}}\frac{1}{x^2+a^2}
\end{equation*}

Use these to find $\sigma_x\sigma_p$.
Note that $\int_{-\infty}^\infty dx/(x^2+a^2)=\pi/a$.
}

\begin{equation*}
\langle x\rangle=\int_{-\infty}^\infty\psi^*x\psi\,dx
=-\frac{a^3}{\pi(x^2+a^2)}\bigg|_{-\infty}^\infty=0
\end{equation*}

Noting that $\arctan(\pm\infty)=\pm\frac{\pi}{2}$ we have
\begin{equation*}
\langle x^2\rangle=\int_{-\infty}^\infty\psi^*x^2\psi\,dx
=\left(\frac{a^2}{\pi}\arctan\frac{x}{a}
-\frac{a^3x}{\pi(x^2+a^2)}\right)\bigg|_{-\infty}^\infty
=a^2
\end{equation*}

\begin{equation*}
\langle p\rangle
=\int_{-\infty}^\infty\psi^*\left(-i\hbar\frac{d}{dx}\psi\right)\,dx
=-\frac{ia^3\hbar}{\pi\left(x^2+a^2\right)^2}\bigg|_{-\infty}^\infty
=0
\end{equation*}

\begin{equation*}
\langle p^2\rangle
=\int_{-\infty}^\infty\psi^*\left(-i\hbar\frac{d}{dx}
\left(-i\hbar\frac{d}{dx}\psi\right)\right)\,dx
=\frac{\hbar^2}{2a^2}
\end{equation*}

\begin{align*}
\sigma_x&=\sqrt{\langle x^2\rangle-\langle x\rangle^2}=a
\\
\sigma_p&=\sqrt{\langle p^2\rangle-\langle p\rangle}
=\frac{\hbar}{a\sqrt2}
\end{align*}

\begin{equation*}
\sigma_x\sigma_p=a\left(\frac{\hbar}{a\sqrt2}\right)
=\frac{\hbar}{\sqrt2}
\end{equation*}

Note that
\begin{equation*}
\sigma_x\sigma_p=\frac{\hbar}{\sqrt2}>\frac{\hbar}{2}
\end{equation*}

\end{document}
