\input{preamble}

\FBOX{
4-10. For a certain system, the operator corresponding
to the physical quantity $A$ does not commute with the Hamiltonian.
It has eigenvalues $a_1$ and $a_2$, corresponding to properly normalized
eigenfunctions
\begin{align*}
\phi_1&=(u_1+u_2)/\sqrt2,
\\
\phi_2&=(u_1-u_2)/\sqrt2,
\end{align*}

where $u_1$ and $u_2$ are properly normalized eigenfunctions of the
Hamiltonian with eigenvalues $E_1$ and $E_2$.
If the system is in state $\psi=\phi_1$ at time $t=0$,
show that the expectation value of $A$ at time $t$ is
\begin{equation*}
\langle A\rangle=\left(\frac{a_1+a_2}{2}\right)
+\left(\frac{a_1-a_2}{2}\right)
\cos\left(\frac{(E_1-E_2)t}{\hbar}\right)
\end{equation*}
}

In matrix form we have
\begin{equation*}
\begin{pmatrix}\phi_1\\\phi_2\end{pmatrix}
=\frac{1}{\sqrt2}
\begin{pmatrix}1&1\\1&-1\end{pmatrix}
\begin{pmatrix}u_1\\u_2\end{pmatrix}
\end{equation*}

Noting that
\begin{equation*}
\begin{pmatrix}1&1\\1&-1\end{pmatrix}^{-1}
=\frac{1}{2}
\begin{pmatrix}1&1\\1&-1\end{pmatrix}
\end{equation*}

we have
\begin{equation*}
\begin{pmatrix}u_1\\u_2\end{pmatrix}
=\frac{1}{\sqrt2}
\begin{pmatrix}1&1\\1&-1\end{pmatrix}
\begin{pmatrix}\phi_1\\\phi_2\end{pmatrix}
\end{equation*}

Hence for $u$ as functions of $\phi$
\begin{align*}
u_1&=(\phi_1+\phi_2)/\sqrt2
\\
u_2&=(\phi_1-\phi_2)/\sqrt2
\end{align*}

By equation (4.162)
\begin{equation*}
\psi(x,t)
=c_1u_1\exp\left(-\frac{iE_1t}{\hbar}\right)
+c_2u_2\exp\left(-\frac{iE_2t}{\hbar}\right)
\end{equation*}

Change to the $\phi$ basis.
\begin{equation*}
\psi(x,t)
=c_1\frac{\phi_1+\phi_2}{\sqrt2}\exp\left(-\frac{iE_1t}{\hbar}\right)
+c_2\frac{\phi_1-\phi_2}{\sqrt2}\exp\left(-\frac{iE_2t}{\hbar}\right)
\end{equation*}

By hypothesis
\begin{equation*}
\phi_1=\psi(x,0)=c_1\frac{\phi_1+\phi_2}{\sqrt2}+c_2\frac{\phi_1-\phi_2}{\sqrt2}
\end{equation*}

Hence
\begin{equation*}
c_1=\frac{1}{\sqrt2},\quad c_2=\frac{1}{\sqrt2}
\end{equation*}

It follows that
\begin{equation*}
\psi
=\frac{\phi_1+\phi_2}{2}\exp\left(-\frac{iE_1t}{\hbar}\right)
+\frac{\phi_1-\phi_2}{2}\exp\left(-\frac{iE_2t}{\hbar}\right)
\end{equation*}

Noting that
\begin{align*}
A\phi_1&=a_1\phi_1
\\
A\phi_2&=a_2\phi_2
\end{align*}

we have
\begin{equation*}
A\psi
=\frac{a_1\phi_1+a_2\phi_2}{2}\exp\left(-\frac{iE_1t}{\hbar}\right)
+\frac{a_1\phi_1-a_2\phi_2}{2}\exp\left(-\frac{iE_2t}{\hbar}\right)
\end{equation*}

Use Eigenmath to verify that
\begin{equation*}
\langle A\rangle
=\int_{-\infty}^\infty \psi^*A\psi\,dx
=\frac{a_1+a_2}{2}+\frac{a_1-a_2}{2}\cos\left(\frac{(E_1-E_2)t}{\hbar}\right)
\end{equation*}

\end{document}
