\input{preamble}

\FBOX{
10.1. Find the Pauli representation of $S_x$, $S_y$, and $S_z$
for a spin-1 particle.
}

For a spin-1 particle we have
\begin{equation*}
s=1,\quad m_s=1,0,-1
\end{equation*}

Let
\begin{equation*}
\chi_{1,1}=\begin{pmatrix}1\\0\\0\end{pmatrix},
\quad
\chi_{1,0}=\begin{pmatrix}0\\1\\0\end{pmatrix},
\quad
\chi_{1,-1}=\begin{pmatrix}0\\0\\1\end{pmatrix}
\end{equation*}

Then by
\begin{equation*}
S_z\chi_{1,1}=\hbar\chi_{1,1},
\quad
S_z\chi_{1,0}=0,
\quad
S_z\chi_{1,-1}=-\hbar\chi_{1,-1}
\end{equation*}

we have
\begin{equation*}
S_z=\hbar\begin{pmatrix}1&0&0\\0&0&0\\0&0&-1\end{pmatrix}
\end{equation*}

For ladder operators we have
\begin{align*}
S_+\chi_{s,m_s}&=c_{s,m_s}^+\chi_{s,m_s+1}
\\
S_-\chi_{s,m_s}&=c_{s,m_s}^-\chi_{s,m_s-1}
\end{align*}

where
\begin{align*}
c_{s,m_s}^+&=\sqrt{s(s+1)-m_s(m_s+1)}\hbar
\\
c_{s,m_s}^-&=\sqrt{s(s+1)-m_s(m_s-1)}\hbar
\end{align*}

It follows that
\begin{equation*}
S_+=\begin{pmatrix}
0 & c_{1,0}^+ & 0
\\
0 & 0 & c_{1,-1}^+
\\
0 & 0 & 0
\end{pmatrix}
=\begin{pmatrix}
0 & \sqrt2\hbar & 0
\\
0 & 0 & \sqrt2\hbar
\\
0 & 0 & 0
\end{pmatrix}
\end{equation*}

and
\begin{equation*}
S_-=\begin{pmatrix}
0 & 0 & 0
\\
c_{1,1}^- & 0 & 0
\\
0 & c_{1,0}^- & 0
\end{pmatrix}
=\begin{pmatrix}
0 & 0 & 0
\\
\sqrt2\hbar & 0 & 0
\\
0 & \sqrt2\hbar & 0
\end{pmatrix}
\end{equation*}

Then by
\begin{equation*}
S_\pm=S_x\pm iS_y
\end{equation*}

we have
\begin{equation*}
S_x=\frac{1}{2}(S_++S_-)
=\frac{\hbar}{\sqrt2}
\begin{pmatrix}
0 & 1 & 0
\\
1 & 0 & 1
\\
0 & 1 & 0
\end{pmatrix}
\end{equation*}

and
\begin{equation*}
S_y=\frac{1}{2i}(S_+-S_-)
=\frac{i\hbar}{\sqrt2}
\begin{pmatrix}
0 & -1 & 0
\\
1 & 0 & -1
\\
0 & 1 & 0
\end{pmatrix}
\end{equation*}

\end{document}
