\input{preamble}

\FBOX{
10.1
Justify Equation (10.5).
}

\begin{equation*}
(\nabla^2+k^2)\psi(\mathbf x)=\frac{2m}{\hbar^2}
\langle\mathbf x|H_1|\psi\rangle
\tag{10.5}
\end{equation*}

Start with equation (10.4).
\begin{equation*}
(H_0+H_1)|\psi\rangle=E|\psi\rangle
\end{equation*}

Rewrite as
\begin{equation*}
H_1|\psi\rangle=-H_0|\psi\rangle+E|\psi\rangle
\end{equation*}

Multiply both sides by $\langle\mathbf x|$.
\begin{equation*}
\langle\mathbf x|H_1|\psi\rangle=-\langle\mathbf x|H_0|\psi\rangle+E\langle\mathbf x|\psi\rangle
\end{equation*}

Noting that in the Schrodinger representation
\begin{equation*}
\langle\mathbf x|H_0|\psi\rangle=-\frac{\hbar^2}{2m}\nabla^2\psi(\mathbf x)
\end{equation*}

we have
\begin{equation*}
\langle\mathbf x|H_1|\psi\rangle=\frac{\hbar^2}{2m}\nabla^2\psi(\mathbf x)
+E\langle\mathbf x|\psi\rangle
\end{equation*}

By equation (10.6)
\begin{equation*}
E=\frac{\hbar^2k^2}{2m}\tag{10.6}
\end{equation*}

and by $\langle\mathbf x|\psi\rangle=\psi(\mathbf x)$ we have
\begin{equation*}
\langle\mathbf x|H_1|\psi\rangle=\frac{\hbar^2}{2m}\nabla^2\psi(\mathbf x)
+\frac{\hbar^2k^2}{2m}\psi(\mathbf x)
\end{equation*}

Multiply both sides by $2m/\hbar^2$.
\begin{equation*}
\frac{2m}{\hbar^2}\langle\mathbf x|H_1|\psi\rangle=\nabla^2\psi(\mathbf x)+k^2\psi(\mathbf x)
\end{equation*}

\end{document}
