\input{preamble}

\FBOX{
10.4
(a) Demonstrate that
\begin{equation*}
\frac{1}{2\pi}\int_{-\infty}^\infty dx\,
\exp\left(-\frac{x^2}{2\sigma_x^2}\right)\cos(kx)
=\frac{1}{(2\pi\sigma_k^2)^{1/2}}\exp\left(-\frac{k^2}{2\sigma_k^2}\right)
\end{equation*}

where $\sigma_k=1/\sigma_x$.

\bigskip
(b) Show that
\begin{equation*}
\frac{1}{(2\pi\sigma_k^2)^{1/2}}
\int_{-\infty}^\infty dk\,\exp\left(-\frac{k^2}{2\sigma_k^2}\right)=1
\end{equation*}

(c) Finally, by taking the limit $\sigma_x\rightarrow\infty$, conclude that
\begin{equation*}
\frac{1}{2\pi}\int_{-\infty}^\infty dx\,\cos(kx)=\delta(x)
\end{equation*}

where $\delta(x)$ is a Dirac delta function.
}

(a) Let
\begin{equation*}
F(k)
=\frac{1}{2\pi}\int_{-\infty}^\infty dx\,
\exp\left(-\frac{x^2}{2\sigma_x^2}\right)\cos(kx)
+\frac{i}{2\pi}\int_{-\infty}^\infty dx\,
\exp\left(-\frac{x^2}{2\sigma_x^2}\right)\sin(kx)
\tag{1}
\end{equation*}

Rewrite as
\begin{equation*}
F(k)=\frac{1}{2\pi}\int_{-\infty}^\infty dx\,
\exp\left(-\frac{x^2}{2\sigma_x^2}+ikx\right)
\end{equation*}

Consider the Gaussian integral
\begin{equation*}
\int_{-\infty}^\infty\exp(-ax^2+bx)\,dx=\sqrt{\frac{\pi}{a}}\exp\left(\frac{b^2}{4a}\right)
\end{equation*}

For $a=1/(2\sigma_x^2)$ and $b=ik$ we have
\begin{equation*}
F(k)=\frac{1}{2\pi}\sqrt{2\pi\sigma_x^2}\exp\left(-\frac{k^2\sigma_x^2}{2}\right)
\end{equation*}

Simplify the coefficient.
\begin{equation*}
F(k)=\sqrt{\frac{\sigma_x^2}{2\pi}}\exp\left(-\frac{k^2\sigma_x^2}{2}\right)
\end{equation*}

Substitute $1/\sigma_k^2$ for $\sigma_x^2$.
\begin{equation*}
F(k)=\frac{1}{\sqrt{2\pi\sigma_k^2}}\exp\left(-\frac{k^2}{2\sigma_k^2}\right)
\tag{2}
\end{equation*}

By equality of the real parts of (1) and (2) we have
\begin{equation*}
\frac{1}{2\pi}\int_{-\infty}^\infty dx\,
\exp\left(-\frac{x^2}{2\sigma_x^2}\right)\cos(kx)
=\frac{1}{\sqrt{2\pi\sigma_k^2}}\exp\left(-\frac{k^2}{2\sigma_k^2}\right)
\end{equation*}

(b) By the well-known Gaussian integral
\begin{equation*}
\int_{-\infty}^\infty\exp(-ax^2)\,dx=\sqrt{\frac{\pi}{a}}
\end{equation*}

with $a=1/(2\sigma_k^2)$ we have
\begin{equation*}
\frac{1}{\sqrt{2\pi\sigma_k^2}}\int_{-\infty}^\infty dk\,\exp\left(-\frac{k^2}{2\sigma_k^2}\right)
=\frac{1}{\sqrt{2\pi\sigma_k^2}}\sqrt{2\pi\sigma_k^2}=1
\end{equation*}

\end{document}
