\input{preamble}

\fbox{\parbox{\dimexpr\linewidth-2\fboxsep-2\fboxrule}{
(37.1)
(a) Verify eqn 37.4.

\bigskip
(b) Show that the rotation matrix
\begin{equation*}
D(\theta^3)=e^{-\tfrac{i}{2}\sigma^3\theta^3}
=\begin{pmatrix}e^{-\frac{i\theta^3}{2}}&0\\0&e^\frac{i\theta^3}{2}\end{pmatrix}
\tag{37.22}
\end{equation*}
}}

\bigskip
(a) This is equation (37.4).
\begin{equation*}
D(\theta^1)=\exp\bigg({-}\frac{i}{2}\sigma^1\theta^1\bigg)
=I\cos\frac{\theta^1}{2}-i\sigma^1\sin\frac{\theta^1}{2}
\tag{37.4}
\end{equation*}

To verify (37.4), start with equation (37.2).
\begin{equation*}
D(\boldsymbol\theta)=\exp\bigg({-}\frac{i}{2}\boldsymbol\sigma\cdot\boldsymbol\theta\bigg)
\tag{37.2}
\end{equation*}

Convert $\boldsymbol\sigma\cdot\boldsymbol\theta$ to component form.
\begin{equation*}
D(\boldsymbol\theta)=\exp\bigg({-}\frac{i}{2}\big(\sigma^1\theta^1+\sigma^2\theta^2+\sigma^3\theta^3\big)\bigg)
\end{equation*}

Then for $\theta^2=\theta^3=0$ we have
\begin{equation*}
D(\theta^1)=\exp\bigg({-}\frac{i}{2}\sigma^1\theta^1\bigg)
\end{equation*}

Convert to rectangular coordinates.
\begin{equation*}
D(\theta^1)=\cos\bigg(\frac{1}{2}\sigma^1\theta^1\bigg)-i\sin\bigg(\frac{1}{2}\sigma^1\theta^1\bigg)
\tag{1}
\end{equation*}

Noting that
\begin{equation*}
\big(\sigma^1\big)^2=\begin{pmatrix}0&1\\1&0\end{pmatrix}\begin{pmatrix}0&1\\1&0\end{pmatrix}
=\begin{pmatrix}1&0\\0&1\end{pmatrix}=I
\end{equation*}
we have
\begin{equation*}
\big(\sigma^1\big)^{2n}=I^n=I
\end{equation*}
and
\begin{equation*}
\big(\sigma^1\big)^{2n+1}=I^{2n}\sigma^1=\sigma^1
\end{equation*}

Hence by considering the Taylor expansion of sine and cosine in (1) we have
\begin{equation*}
D(\theta^1)=I\cos\frac{\theta^1}{2}-i\sigma^1\sin\frac{\theta^1}{2}
\end{equation*}

(b) Note that
\begin{equation*}
\big(\sigma^3\big)^2=\begin{pmatrix}1&0\\0&-1\end{pmatrix}\begin{pmatrix}1&0\\0&-1\end{pmatrix}
=\begin{pmatrix}1&0\\0&1\end{pmatrix}=I
\end{equation*}

Hence by the same argument as in part (a) we have
\begin{equation*}
D(\theta^3)=I\cos\frac{\theta^3}{2}-i\sigma^3\sin\frac{\theta^3}{2}
\end{equation*}

Rewrite in matrix form.
\begin{equation*}
D(\theta^3)
=\begin{pmatrix}
\cos\frac{\theta^3}{2}-i\sin\frac{\theta^3}{2}&0
\\
0&\cos\frac{\theta^3}{2}+i\sin\frac{\theta^3}{2}&0
\end{pmatrix}
=\begin{pmatrix}e^{-\frac{i\theta^3}{2}}&0\\0&e^\frac{i\theta^3}{2}\end{pmatrix}
\end{equation*}

\end{document}
