\input{preamble}

\fbox{\parbox{\dimexpr\linewidth-2\fboxsep-2\fboxrule}{
(37.2)
Show that both choices of sign $\mathbf K=\pm\frac{i\boldsymbol\sigma}{2}$ obey the
necessary commutation relations.
}}

\bigskip
These are the commutation relations from page 336.
\begin{align*}
[J^i,K^j]&=i\varepsilon^{ijk}K^k
\\
[K^i,K^j]&=-i\varepsilon^{ijk}J^k
\end{align*}

On page 337 we are given
\begin{equation*}
\mathbf J=\tfrac{1}{2}\boldsymbol\sigma
\end{equation*}
and
\begin{equation*}
[\sigma^i,\sigma^j]=2i\varepsilon^{ijk}\sigma^k
\tag{1}
\end{equation*}

For the first commutation relation we have
\begin{equation*}
[J^i,\pm K^j]
=\big[\tfrac{1}{2}\sigma^i,\pm\tfrac{i}{2}\sigma^j\big]
=\pm\tfrac{i}{4}[\sigma^i,\sigma^j]
\end{equation*}

By equation (1)
\begin{equation*}
\pm\tfrac{i}{4}[\sigma^i,\sigma^j]
=\pm\tfrac{i}{4}\big(2i\varepsilon^{ijk}\sigma^k\big)
=\mp\tfrac{1}{2}\varepsilon^{ijk}\sigma^k
=\pm i\varepsilon^{ijk}K^k
\end{equation*}

For the second commutation relation we have
\begin{equation*}
[K^i,K^j]=\big[\tfrac{i}{2}\sigma^i,\tfrac{i}{2}\sigma^j\big]
=\big[{-}\tfrac{i}{2}\sigma^i,-\tfrac{i}{2}\sigma^j\big]
=-\tfrac{1}{4}[\sigma^i,\sigma^j]
\end{equation*}

By equation (1)
\begin{equation*}
-\tfrac{1}{4}[\sigma^i,\sigma^j]
=-\tfrac{1}{4}\big(2i\varepsilon^{ijk}\sigma^k\big)
=-i\varepsilon^{ijk}J^k
\end{equation*}

\end{document}

Recall that $\varepsilon^{ijk}$ is the Levi-Civita symbol
\begin{equation*}
\varepsilon^1=\begin{pmatrix}
0&0&0
\\
0&0&1
\\
0&-1&0
\end{pmatrix},
\quad
\varepsilon^2=\begin{pmatrix}
0&0&-1
\\
0&0&0
\\
1&0&0
\end{pmatrix},
\quad
\varepsilon^3=\begin{pmatrix}
0&1&0
\\
-1&0&0
\\
0&0&0
\end{pmatrix}
\end{equation*}

\end{document}
